src/Util.v
@@ -1,0 +1,24 @@
+Require Import List.
+Open Scope list_scope.
+
+Lemma list_Forall_map : forall X Y (P : Y -> Prop) (f : X -> Y) l,
+  Forall P (map f l) <-> Forall (fun x => P (f x)) l.
+Proof.
+Admitted.
+
+Lemma list_Exists_map : forall X Y (P : Y -> Prop) (f : X -> Y) l,
+  Exists P (map f l) <-> Exists (fun x => P (f x)) l.
+Proof.
+Admitted.
+
+Lemma list_Exists_Forall_and : forall X (P Q: X -> Prop) l,
+    Exists P l ->
+    Forall Q l ->
+    Exists (fun x => P x /\ Q x) l.
+Proof.
+  intros X P Q l ex all.
+  rewrite (Exists_exists P l) in ex. destruct ex as [x [x_in px]].
+  rewrite Exists_exists. exists x.
+  rewrite Forall_forall in all.
+  split; [|split]; now auto.
+Qed.
